src/proof/index.v
@@ -18,19 +18,19 @@ Context `{!mapG Σ KKey.t (gset KKey.t)}.
 Context `{!auth_setG Σ KKey.t}.
 
 (* TODO: revisit this spec *)
-Lemma wp_State__ByIndex_pod l kind index_name indexed_value
-  γ_state γ_children γ_fresh_keys parent_key owned_parent owned_pod_map owned_child_keys:
+Lemma wp_State__ByIndex_pod γ l kind index_name indexed_value
+  parent_key owned_parent owned_pod_map owned_child_keys:
   {{{ is_pkg_init apimodel ∗
-      "#Hisk" ∷ is_kubernetes γ_state γ_children γ_fresh_keys l ∗
+      "#Hisk" ∷ is_kubernetes γ l ∗
       "%Hkind" ∷ ⌜ kind = "Pod"%go ⌝ ∗
       "%Hindex_name" ∷ ⌜ index_name = "podController"%go ⌝ ∗
       "%Hindexed_value" ∷ ⌜ indexed_value = parent_key.(KKey.Namespace') ++ "/"%go ++
                                             parent_key.(KKey.Kind') ++ "/"%go ++
                                             parent_key.(KKey.Name') ++ "/"%go ++
                                             (PureKObject.metadata owned_parent).(PureObjectMeta.UID') ⌝ ∗
-      "Hown_parent" ∷ parent_key [[ γ_state ]]↦ owned_parent ∗
-      "Hown_pods" ∷ ([∗ map] key ↦ pod ∈ owned_pod_map, key [[ γ_state ]]↦ PureKObject.Pod pod) ∗
-      "Hown_child_keys" ∷ parent_key [[ γ_children ]]↦ owned_child_keys ∗
+      "Hown_parent" ∷ parent_key [[ γ.(γ_state) ]]↦ owned_parent ∗
+      "Hown_pods" ∷ ([∗ map] key ↦ pod ∈ owned_pod_map, key [[ γ.(γ_state) ]]↦ PureKObject.Pod pod) ∗
+      "Hown_child_keys" ∷ parent_key [[ γ.(γ_children) ]]↦ owned_child_keys ∗
       "%Hdom_eq" ∷ ⌜ owned_child_keys = dom owned_pod_map ⌝
   }}}
     l @ (ptrT.id apimodel.State.id) @ "ByIndex" #kind #index_name #indexed_value
@@ -41,9 +41,9 @@ Lemma wp_State__ByIndex_pod l kind index_name indexed_value
       "%Hwell_formed_pure_pods" ∷ ⌜ ∀ pure_pod, pure_pod ∈ pure_pods → PurePod.well_formed pure_pod ⌝ ∗
       "%Hlen_pure_pods" ∷ ⌜ length pure_pods = size owned_pod_map ⌝ ∗
       "%Hkey_set_equal_dom_owned_pods" ∷  ⌜ ∀ pure_pod, pure_pod ∈ pure_pods → ∃ k, owned_pod_map !! k = Some pure_pod ⌝ ∗
-      "Hown_parent" ∷ parent_key [[ γ_state ]]↦ owned_parent ∗
-      "Hown_pods" ∷ ([∗ map] key ↦ pod ∈ owned_pod_map, key [[ γ_state ]]↦ PureKObject.Pod pod) ∗
-      "Hown_child_keys" ∷ parent_key [[ γ_children ]]↦ owned_child_keys
+      "Hown_parent" ∷ parent_key [[ γ.(γ_state) ]]↦ owned_parent ∗
+      "Hown_pods" ∷ ([∗ map] key ↦ pod ∈ owned_pod_map, key [[ γ.(γ_state) ]]↦ PureKObject.Pod pod) ∗
+      "Hown_child_keys" ∷ parent_key [[ γ.(γ_children) ]]↦ owned_child_keys
   }}}.
 Proof.
 Admitted.
